frodo/code/Hacl.Impl.Frodo.Params.fst
@@ -3,21 +3,23 @@ module Hacl.Impl.Frodo.Params
 open Lib.IntTypes
 open Lib.PQ.Buffer
 
-let params_n = size 64 // 640
+module S = Spec.Frodo.Params
 
-let params_logq = size 15
+let params_n: r:size_t{v r = S.params_n} = size 64 // 640
 
-let params_extracted_bits = size 2
+let params_logq: r:size_t{v r = S.params_logq} = size 15
 
-let crypto_bytes = size 16
+let params_extracted_bits: r:size_t{v r = S.params_extracted_bits} = size 2
 
-let cdf_table_len = size 12
+let crypto_bytes: r:size_t{v r = S.crypto_bytes} = size 16
+
+let cdf_table_len: r:size_t{v r = S.cdf_table_len} = size 12
 
 let cdf_table: b:lbuffer uint16 (v cdf_table_len) { LowStar.Buffer.recallable b } =
   LowStar.Buffer.gcmalloc_of_list HyperStack.root
     [u16 4727; u16 13584; u16 20864; u16 26113; u16 29434; u16 31278;
      u16 32176; u16 32560; u16 32704; u16 32751; u16 32764; u16 32767]
 
-let bytes_seed_a = size 16
+let bytes_seed_a: r:size_t{v r = S.bytes_seed_a} = size 16
 
-let params_nbar = size 8
+let params_nbar:r:size_t{v r = S.params_nbar} = size 8
